Compile simplified conf rels to simplified first order logic.

deps/poulet4/lib/P4automata/CompileConfRelSimplified.v
@@ -23,8 +23,6 @@ Section CompileConfRelSimplified.
 
   Variable (a: P4A.t S H).
 
-  Notation conf := (configuration (P4A.interp a)).
-
   Fixpoint compile_bctx (b: bctx): ctx (sig a) :=
     match b with
     | BCEmp => CEmp _
@@ -52,159 +50,150 @@ Section CompileConfRelSimplified.
   Proof.
   Admitted.
 
+  Definition outer_ctx b1 b2 :=
+    CSnoc (sig a) (
+      CSnoc (sig a) (
+        CSnoc (sig a) (
+          CSnoc (sig a) (CEmp (sig a)) Store
+        ) Store
+      ) (Bits b2)
+    ) (Bits b1).
+
+  Definition var_buf1 b1 b2 : var (sig a) (outer_ctx b1 b2) (Bits b1) :=
+    VHere (sig a) _ _.
+
+  Definition var_buf2 b1 b2 : var (sig a) (outer_ctx b1 b2) (Bits b2) :=
+    VThere (sig a) _ _ _ (VHere (sig a) _ _).
+
+  Definition var_store1 b1 b2 : var (sig a) (outer_ctx b1 b2) Store :=
+    VThere (sig a) _ _ _ (VThere (sig a) _ _ _ (VHere (sig a) _ _)).
+
+  Definition var_store2 b1 b2 : var (sig a) (outer_ctx b1 b2) Store :=
+    VThere (sig a) _ _ _ (VThere (sig a) _ _ _ (
+    VThere (sig a) _ _ _ (VHere (sig a) _ _))).
+
+  Definition outer_valu {b1 b2} buf1 buf2 store1 store2 :=
+    VSnoc _ (fm_model a) (Bits b1) _ buf1 (
+    VSnoc _ (fm_model a) (Bits b2) _ buf2 (
+    VSnoc _ (fm_model a) Store _ store1 (
+    VSnoc _ (fm_model a) Store _ store2 (
+    VEmp _ _)))).
+
   Equations compile_bit_expr
             {c: bctx}
-            {b1 b2: nat}
-            (buf1: tm (sig a) (compile_bctx c) (Bits b1))
-            (buf2: tm (sig a) (compile_bctx c) (Bits b2))
-            (store1 store2: tm (sig a) (compile_bctx c) Store)
+            (b1 b2: nat)
             (e: bit_expr H c)
-    : tm (sig a) (compile_bctx c) (be_sort b1 b2 e) :=
-    { compile_bit_expr buf1 buf2 store1 store2 (BELit _ _ l) :=
+    : tm (sig a) (app_ctx (outer_ctx b1 b2) (compile_bctx c)) (be_sort b1 b2 e) :=
+    { compile_bit_expr b1 b2 (BELit _ _ l) :=
         TFun (sig a) (BitsLit _ (List.length l) (Ntuple.l2t l)) TSNil;
-      compile_bit_expr buf1 buf2 store1 store2 (BEBuf _ _ Left) := buf1;
-      compile_bit_expr buf1 buf2 store1 store2 (BEBuf _ _ Right) := buf2;
-      compile_bit_expr buf1 buf2 store1 store2 (@BEHdr H _ Left (P4A.HRVar h)) :=
+      compile_bit_expr b1 b2 (BEBuf _ _ Left) :=
+        TVar (weaken_var _ (var_buf1 b1 b2));
+      compile_bit_expr b1 b2 (BEBuf _ _ Right) :=
+        TVar (weaken_var _ (var_buf2 b1 b2));
+      compile_bit_expr b1 b2 (@BEHdr H _ Left (P4A.HRVar h)) :=
         let key := TFun (sig a) (KeyLit _ _ (projT2 h)) TSNil in
-        TFun (sig a) (Lookup _ (projT1 h)) (TSCons store1 (TSCons key TSNil));
-      compile_bit_expr buf1 buf2 store1 store2 (BEHdr _ Right (P4A.HRVar h)) :=
+        TFun (sig a) (Lookup _ (projT1 h))
+             (TSCons (TVar (weaken_var _ (var_store1 b1 b2))) (TSCons key TSNil));
+      compile_bit_expr b1 b2 (BEHdr _ Right (P4A.HRVar h)) :=
         let key := TFun (sig a) (KeyLit _ _ (projT2 h)) TSNil in
-        TFun (sig a) (Lookup _ (projT1 h)) (TSCons store2 (TSCons key TSNil));
-      compile_bit_expr buf1 buf2 store1 store2 (BEVar _ b) :=
-        TVar (compile_var b);
-      compile_bit_expr buf1 buf2 store1 store2 (BESlice e hi lo) :=
+        TFun (sig a) (Lookup _ (projT1 h))
+             (TSCons (TVar (weaken_var _ (var_store1 b1 b2))) (TSCons key TSNil));
+      compile_bit_expr b1 b2 (BEVar _ b) :=
+        TVar (reindex_var (compile_var b));
+      compile_bit_expr b1 b2 (BESlice e hi lo) :=
         TFun (sig a) (Slice _ _ hi lo)
-             (TSCons (compile_bit_expr buf1 buf2 store1 store2 e) TSNil);
-      compile_bit_expr buf1 buf2 store1 store2 (BEConcat e1 e2) :=
+             (TSCons (compile_bit_expr b1 b2 e) TSNil);
+      compile_bit_expr b1 b2 (BEConcat e1 e2) :=
         TFun (sig a) (Concat _ _ _)
-             (TSCons (compile_bit_expr buf1 buf2 store1 store2 e1)
-             (TSCons (compile_bit_expr buf1 buf2 store1 store2 e2) TSNil)) }.
+             (TSCons (compile_bit_expr b1 b2 e1)
+             (TSCons (compile_bit_expr b1 b2 e2) TSNil)) }.
 
   Equations compile_store_rel
             {c: bctx}
-            {b1 b2: nat}
-            (buf1: tm (sig a) (compile_bctx c) (Bits b1))
-            (buf2: tm (sig a) (compile_bctx c) (Bits b2))
-            (store1 store2: tm (sig a) (compile_bctx c) Store)
+            (b1 b2: nat)
             (r: store_rel H c)
-            : fm (sig a) (compile_bctx c) :=
-    { compile_store_rel buf1 buf2 store1 store2 BRTrue := FTrue;
-      compile_store_rel buf1 buf2 store1 store2 BRFalse := FFalse;
-      compile_store_rel buf1 buf2 store1 store2 (BREq e1 e2) :=
+            : fm (sig a) (app_ctx (outer_ctx b1 b2) (compile_bctx c)) :=
+    { compile_store_rel b1 b2 BRTrue := FTrue;
+      compile_store_rel b1 b2 BRFalse := FFalse;
+      compile_store_rel b1 b2 (BREq e1 e2) :=
         match eq_dec (be_size b1 b2 e1) (be_size b1 b2 e2) with
         | left Heq =>
           FEq (eq_rect _ (fun n => tm (sig a) _ (Bits n))
-                       (compile_bit_expr buf1 buf2 store1 store2 e1) _ Heq)
-              (compile_bit_expr buf1 buf2 store1 store2 e2)
+                       (compile_bit_expr b1 b2 e1) _ Heq)
+              (compile_bit_expr b1 b2 e2)
         | right _ => FFalse
         end;
-      compile_store_rel buf1 buf2 store1 store2 (BRAnd r1 r2) :=
-        FAnd _ (compile_store_rel buf1 buf2 store1 store2 r1)
-               (compile_store_rel buf1 buf2 store1 store2 r2);
-      compile_store_rel buf1 buf2 store1 store2 (BROr r1 r2) :=
-        FOr _ (compile_store_rel buf1 buf2 store1 store2 r1)
-              (compile_store_rel buf1 buf2 store1 store2 r2);
-      compile_store_rel buf1 buf2 store1 store2 (BRImpl r1 r2) :=
-        FOr _ (FNeg _ (compile_store_rel buf1 buf2 store1 store2 r1))
-              (compile_store_rel buf1 buf2 store1 store2 r2)
+      compile_store_rel b1 b2 (BRAnd r1 r2) :=
+        FAnd _ (compile_store_rel b1 b2 r1)
+               (compile_store_rel b1 b2 r2);
+      compile_store_rel b1 b2 (BROr r1 r2) :=
+        FOr _ (compile_store_rel b1 b2 r1)
+              (compile_store_rel b1 b2 r2);
+      compile_store_rel b1 b2 (BRImpl r1 r2) :=
+        FOr _ (FNeg _ (compile_store_rel b1 b2 r1))
+              (compile_store_rel b1 b2 r2)
     }.
 
   Definition compile_simplified_conf_rel
-    {b1 b2: nat}
+    (b1 b2: nat)
     (r: simplified_conf_rel H)
-    (buf1: tm (sig a) (CEmp _) (Bits b1))
-    (buf2: tm (sig a) (CEmp _) (Bits b2))
-    (store1 store2: tm (sig a) (CEmp _) Store)
-    : fm (sig a) (CEmp _)
+    : fm (sig a) (outer_ctx b1 b2)
   :=
     let sr: fm (sig a) _ :=
-        (compile_store_rel (reindex_tm buf1)
-                           (reindex_tm buf2)
-                           (reindex_tm store1)
-                           (reindex_tm store2)
-                           (projT2 r))
+        compile_store_rel b1 b2 (projT2 r)
     in
-    quantify_all _ sr.
+    quantify _ sr.
 
   Definition compile_simplified_crel
-    {b1 b2: nat}
+    (b1 b2: nat)
     (R: simplified_crel H)
-    (buf1: tm (sig a) (CEmp _) (Bits b1))
-    (buf2: tm (sig a) (CEmp _) (Bits b2))
-    (store1 store2: tm (sig a) (CEmp _) Store)
-    : fm (sig a) (CEmp _) :=
+    : fm (sig a) (outer_ctx b1 b2) :=
     List.fold_right (fun r f =>
-      FAnd _ (compile_simplified_conf_rel r buf1 buf2 store1 store2) f
+      FAnd _ (compile_simplified_conf_rel b1 b2 r) f
     ) FTrue R.
 
   Definition compile_simplified_entailment
     (se: simplified_entailment a)
-    (buf1: tm (sig a) (CEmp _) (Bits se.(se_st).(cs_st1).(st_buf_len)))
-    (buf2: tm (sig a) (CEmp _) (Bits se.(se_st).(cs_st2).(st_buf_len)))
-    (store1 store2: tm (sig a) (CEmp _) Store)
     : fm (sig a) (CEmp _) :=
-    (FImpl (compile_simplified_crel se.(se_prems) buf1 buf2 store1 store2)
-           (compile_simplified_conf_rel se.(se_concl) buf1 buf2 store1 store2)).
-
-  Definition compile_buf
-    {c': ctx (sig a)}
-    {n: nat}
-    (buf: n_tuple bool n)
-    : tm (sig a) c' (Bits n) :=
-    TFun (sig a) (BitsLit _ _ buf) TSNil.
-
-  Definition compile_store
-    {c': ctx (sig a)}
-    (store: store (P4A.interp a))
-    : tm (sig a) c' Store :=
-    TFun (sig a) (StoreLit store) TSNil.
+    quantify_all _
+      (FImpl (compile_simplified_crel
+               se.(se_st).(cs_st1).(st_buf_len)
+               se.(se_st).(cs_st2).(st_buf_len)
+               se.(se_prems))
+             (compile_simplified_conf_rel
+               se.(se_st).(cs_st1).(st_buf_len)
+               se.(se_st).(cs_st2).(st_buf_len)
+               se.(se_concl))).
 
   Lemma compile_store_rel_correct:
-    forall c (r: store_rel H c) valu b1 b2 (buf1: n_tuple bool b1) (buf2: n_tuple bool b2) store1 store2,
-      interp_store_rel r valu buf1 buf2 store1 store2 <->
-      interp_fm (m := fm_model a) (compile_bval valu)
-                (compile_store_rel (compile_buf buf1)
-                                   (compile_buf buf2)
-                                   (compile_store store1)
-                                   (compile_store store2) r).
+    forall c (r: store_rel H c) bval b1 b2 buf1 buf2 store1 store2,
+      interp_store_rel r bval buf1 buf2 store1 store2 <->
+      let valu := outer_valu buf1 buf2 store1 store2 in
+      interp_fm (m := fm_model a) (app_valu _ valu (compile_bval bval))
+                (compile_store_rel b1 b2 r).
   Proof.
   Admitted.
 
   Lemma compile_simplified_conf_rel_correct:
-    forall r b1 b2 (buf1: n_tuple bool b1) (buf2: n_tuple bool b2) store1 store2,
+    forall r b1 b2 buf1 buf2 store1 store2,
       interp_simplified_conf_rel r buf1 buf2 store1 store2 <->
-      interp_fm (m := fm_model a) (VEmp _ _)
-                (compile_simplified_conf_rel r
-                  (compile_buf buf1)
-                  (compile_buf buf2)
-                  (compile_store store1)
-                  (compile_store store2)).
+      interp_fm (m := fm_model a) (outer_valu buf1 buf2 store1 store2)
+                (compile_simplified_conf_rel b1 b2 r).
   Proof.
   Admitted.
 
   Lemma compile_crel_correct:
-    forall r b1 b2 (buf1: n_tuple bool b1) (buf2: n_tuple bool b2) store1 store2,
+    forall r b1 b2 buf1 buf2 store1 store2,
       interp_simplified_crel r buf1 buf2 store1 store2 <->
-      interp_fm (m := fm_model a) (VEmp _ _)
-                (compile_simplified_crel r
-                  (compile_buf buf1)
-                  (compile_buf buf2)
-                  (compile_store store1)
-                  (compile_store store2)).
+      interp_fm (m := fm_model a) (outer_valu buf1 buf2 store1 store2)
+                (compile_simplified_crel b1 b2 r).
   Proof.
   Admitted.
 
   Lemma compile_simplified_entailment_correct:
       forall i e,
         interp_simplified_entailment i e <->
-        forall buf1 buf2 store1 store2,
-          interp_fm (m := fm_model a)
-                  (VEmp _ _)
-                  (compile_simplified_entailment e
-                    (compile_buf buf1)
-                    (compile_buf buf2)
-                    (compile_store store1)
-                    (compile_store store2)).
+        interp_fm (m := fm_model a) (VEmp _ _) (compile_simplified_entailment e).
   Proof.
   Admitted.
 
